

proofs of Lemmas

Rohan Senapati

July 2025

1 Introduction

1.0.1 Rotational Symmetries

In the rotational case, which is easier than the reflectional case, we can actually prove Lemma 4 directly. The first step of the rotational symmetry proofs is to assign ω to a $j - 1^{th}$ root of unity. We then proceed to iterate ω over the polynomial $f(z) = z^j + c$. After a few iterations, we observe that each iterate rotates the previous one by ω .

Proof of Lemma 4 Case 4

$$\underline{f(z) = z^4 + c}$$

$$\text{Let } \omega = e^{2\pi i/3}$$

$$f(z) = z^4 + \omega c$$

$$f(0) = 0^4 + \omega c = \omega c$$

$$f(\omega c) = (\omega c)^4 + \omega c$$

$$\omega^3 = 1 \rightarrow \omega^4 = \omega$$

$$\rightarrow f(\omega c) = \omega c^4 + \omega c$$

$$= \omega(c^4 + c)$$

$$f(\omega(c^4 + c)) = (\omega(c^4 + c))^4 + \omega c$$

$$= \omega^4(c^4 + c)^4 + \omega c$$

$$= \omega(c^4 + c)^4 + \omega c$$

$$= \omega[(c^4 + c)^4 + c]$$

Proof of Lemma 4 Case 9

$$\underline{f(z) = z^5 + c}$$

$$\text{Let } \omega = e^{2\pi i/4}$$

$$\rightarrow \omega = i$$

$$f(z) = z^5 + ic$$

$$f(0) = 0^5 + ic = ic$$

$$f(ic) = (ic)^5 + ic$$

$$i^4 = 1 \rightarrow i^5 = i \text{ or } \omega^4 = 1 \rightarrow \omega^5 = \omega$$

$$(ic)^5 = i^5 * c^5 = ic^5$$

$$\rightarrow f(ic) = ic^5 + ic$$

$$= i(c^5 + c)$$

$$f(i(c^5 + c)) = (i(c^5 + c))^5 + ic$$

$$= i^5(c^5 + c)^5 + ic$$

$$= i(c^5 + c)^5 + ic$$

$$= i[(c^5 + c)^5 + c]$$

Proof of Lemma 4 Case 11

$$\underline{f(z) = z^6 + c}$$

$$\text{Let } \omega = e^{2\pi i/5}$$

$$f(z) = z^6 + \omega c$$

$$f(0) = 0^6 + \omega c = \omega c$$

$$f(\omega c) = (\omega c)^6 + \omega c$$

$$\omega^5 = 1 \rightarrow \omega^6 = \omega$$

$$\rightarrow f(\omega c) = \omega c^6 + \omega c$$

$$= \omega(c^6 + c)$$

$$f(\omega(c^6 + c)) = (\omega(c^6 + c))^6 + \omega c$$

$$= \omega^6(c^6 + c)^6 + \omega c$$

$$= \omega(c^6 + c)^6 + \omega c$$

$$= \omega[(c^6 + c)^6 + c]$$

Note : For rotations, Lemma 2 is immediately clear by taking absolute values.

Disclaimer : After completing our work, we were informed that Cases 4, 9, and 11 of this lemma are also proved in the blog of Inigo Quilez [12], who is known for their beautiful mathematical visualizations.

1.0.2 Reflectional Symmetries

The next 16 cases regarding reflectional symmetry (from Lemmas 2 and 3) are proved by writing the formula for the reflection R in (x, y) form. Using Wolfram Alpha, we checked some of the longer computations in this section.

1.0.3 $f(z) = z^4 + c$

$y = -\sqrt{3}x$

$$R(x, y) = \left(\frac{(1 - (-\sqrt{3})^2)x + 2(-\sqrt{3})y}{1 + (-\sqrt{3})^2}, \frac{((- \sqrt{3})^2 - 1)y + 2(-\sqrt{3})x}{1 + (-\sqrt{3})^2} \right)$$

$$R(x, y) = \left(-\frac{1}{2}x - \frac{\sqrt{3}}{2}y, -\frac{\sqrt{3}}{2}x + \frac{1}{2}y \right)$$

Proof of Lemma 2 Case 1

Let $z = a + bi$; (a, b)

$$R(z)$$

$$= R(a, b)$$

$$= \left(-\frac{1}{2}a - \frac{\sqrt{3}}{2}b, -\frac{\sqrt{3}}{2}a + \frac{1}{2}b \right)$$

$$\begin{aligned} & |R(z)| \\ &= \sqrt{\left(-\frac{1}{2}a - \frac{\sqrt{3}}{2}b \right)^2 + \left(-\frac{\sqrt{3}}{2}a + \frac{1}{2}b \right)^2} \\ &= \sqrt{a^2 + b^2} \\ &= |z| \end{aligned}$$

$$|R(z)| = |z|$$

Proof of Lemma 3 Case 1

$$z^4 = (a^4 - 6a^2b^2 + b^4, 4a^3b - 4ab^3)$$

$$\begin{aligned} & R(z^4) \\ &= R(a^4 - 6a^2b^2 + b^4, 4a^3b - 4ab^3) \\ &= \left(-\frac{1}{2}(a^4 - 6a^2b^2 + b^4) - \frac{\sqrt{3}}{2}(4a^3b - 4ab^3), -\frac{\sqrt{3}}{2}(a^4 - 6a^2b^2 + b^4) + \frac{1}{2}(4a^3b - 4ab^3) \right) \\ &= \left[-\frac{1}{2}(a^4 - 6a^2b^2 + b^4) - \frac{\sqrt{3}}{2}(4a^3b - 4ab^3) \right] + \left[-\frac{\sqrt{3}}{2}(a^4 - 6a^2b^2 + b^4) + \frac{1}{2}(4a^3b - 4ab^3) \right]i \end{aligned}$$

$$\begin{aligned} & (R(z))^4 \\ & R(z) \\ &= R(a, b) \\ &= \left(-\frac{1}{2}a - \frac{\sqrt{3}}{2}b, -\frac{\sqrt{3}}{2}a + \frac{1}{2}b \right) \\ &= \left[-\frac{1}{2}a - \frac{\sqrt{3}}{2}b \right] + \left[-\frac{\sqrt{3}}{2}a + \frac{1}{2}b \right]i \\ & (R(z))^4 \\ &= \left(\left[-\frac{1}{2}a - \frac{\sqrt{3}}{2}b \right] + \left[-\frac{\sqrt{3}}{2}a + \frac{1}{2}b \right]i \right)^4 \end{aligned}$$

$$= [-\frac{1}{2}(a^4 - 6a^2b^2 + b^4) - \frac{\sqrt{3}}{2}(4a^3b - 4ab^3)] + [-\frac{\sqrt{3}}{2}(a^4 - 6a^2b^2 + b^4) + \frac{1}{2}(4a^3b - 4ab^3))]i$$

$$= R(z^4)$$

$$R(z^4) = (R(z))^4$$

$$y = \sqrt{3}x$$

$$R(x, y) = (\frac{(1-(\sqrt{3})^2)x+2(\sqrt{3})y}{1+(\sqrt{3})^2}, \frac{((\sqrt{3})^2-1)y+2(\sqrt{3})x}{1+(\sqrt{3})^2})$$

$$R(x, y) = (-\frac{1}{2}x + \frac{\sqrt{3}}{2}y, \frac{\sqrt{3}}{2}x + \frac{1}{2}y)$$

Proof of Lemma 2 Case 2

Let $z = a + bi$; (a, b)

$$R(z)$$

$$= R(a, b)$$

$$= (-\frac{1}{2}a + \frac{\sqrt{3}}{2}b, \frac{\sqrt{3}}{2}a + \frac{1}{2}b)$$

$$|R(z)|$$

$$= \sqrt{(-\frac{1}{2}a + \frac{\sqrt{3}}{2}b)^2 + (\frac{\sqrt{3}}{2}a + \frac{1}{2}b)^2}$$

$$= \sqrt{a^2 + b^2}$$

$$= |z|$$

$$|R(z)| = |z|$$

Proof of Lemma 3 Case 2

$$z^4 = (a + bi)^4 = a^4 + 4a^3bi - 6a^2b^2 - 4ab^3i + b^4$$

$$= (a^4 - 6a^2b^2 + b^4) + (4a^3b - 4ab^3)i$$

$$= (a^4 - 6a^2b^2 + b^4, 4a^3b - 4ab^3)$$

$$R(z^4)$$

$$= R(a^4 - 6a^2b^2 + b^4, 4a^3b - 4ab^3)$$

$$= (-\frac{1}{2}(a^4 - 6a^2b^2 + b^4) + \frac{\sqrt{3}}{2}(4a^3b - 4ab^3), \frac{\sqrt{3}}{2}(a^4 - 6a^2b^2 + b^4) + \frac{1}{2}(4a^3b - 4ab^3))$$

$$= [-\frac{1}{2}(a^4 - 6a^2b^2 + b^4) + \frac{\sqrt{3}}{2}(4a^3b - 4ab^3)] + [\frac{\sqrt{3}}{2}(a^4 - 6a^2b^2 + b^4) + \frac{1}{2}(4a^3b - 4ab^3))]i$$

$$(R(z))^4$$

$$R(z)$$

$$= R(a, b)$$

$$= (-\frac{1}{2}a + \frac{\sqrt{3}}{2}b, \frac{\sqrt{3}}{2}a + \frac{1}{2}b)$$

$$= [-\frac{1}{2}a + \frac{\sqrt{3}}{2}b] + [\frac{\sqrt{3}}{2}a + \frac{1}{2}b]i$$

$$(R(z))^4$$

$$\begin{aligned}
&= \left(\left[-\frac{1}{2}a + \frac{\sqrt{3}}{2}b \right] + \left[\frac{\sqrt{3}}{2}a + \frac{1}{2}b \right] i \right)^4 \\
&= \left[-\frac{1}{2}(a^4 - 6a^2b^2 + b^4) + \frac{\sqrt{3}}{2}(4a^3b - 4ab^3) \right] + \left[\frac{\sqrt{3}}{2}(a^4 - 6a^2b^2 + b^4) + \frac{1}{2}(4a^3b - 4ab^3) \right] i \\
&= R(z^4)
\end{aligned}$$

$$R(z^4) = (R(z))^4$$

$$\underline{y = 0}$$

$$R(x, y) = \left(\frac{(1-(0)^2)x+2(0)y}{1+(0)^2}, \frac{((0)^2-1)y+2(0)x}{1+(0)^2} \right)$$

$$R(x, y) = (x, -y)$$

Proof of Lemma 2 Case 3

$$\begin{aligned}
&\text{Let } z = a + bi; (a, b) \\
&R(z) = R(a, b) = (a, -b)
\end{aligned}$$

$$\begin{aligned}
&|R(z)| = |(a, -b)| \\
&= \sqrt{a^2 + (-b)^2} \\
&= \sqrt{a^2 + b^2} \\
&= |z|
\end{aligned}$$

$$|R(z)| = |z|$$

Proof of Lemma 3 Case 3

$$z^4 = (a^4 - 6a^2b^2 + b^4, 4a^3b - 4ab^3)$$

$$\begin{aligned}
&R(z^4) \\
&= R(a^4 - 6a^2b^2 + b^4, 4a^3b - 4ab^3) \\
&= (a^4 - 6a^2b^2 + b^4, -[4a^3b - 4ab^3]) \\
&= [a^4 - 6a^2b^2 + b^4] + [-(4a^3b - 4ab^3)]i
\end{aligned}$$

$$\begin{aligned}
&(R(z))^4 \\
&= [a + (-b)i]^4 \\
&= [a^4 - 6a^2b^2 + b^4] + [-(4a^3b - 4ab^3)]i \\
&= R(z^4)
\end{aligned}$$

$$R(z^4) = (R(z))^4$$

$$\mathbf{1.0.4} \quad f(z) = z^5 + c$$

$$\underline{y = x}$$

$$R(x, y) = \left(\frac{(1-(1)^2)x+2(1)y}{1+(1)^2}, \frac{((1)^2-1)y+2(1)x}{1+(1)^2} \right)$$

$$R(x, y) = (y, x)$$

Proof of Lemma 2 Case 5

Let $z = a + bi; (a, b)$

$$\begin{aligned} R(z) \\ &= R(a, b) \\ &= (b, a) \end{aligned}$$

$$\begin{aligned} |R(z)| \\ &= |(b, a)| \\ &= \sqrt{b^2 + a^2} \\ &= \sqrt{a^2 + b^2} \\ &= |z| \end{aligned}$$

$$|R(z)| = |z|$$

Proof of Lemma 3 Case 5

$$\begin{aligned} z^5 &= (a + bi)^5 \\ &= a^5 + 5a^4bi - 10a^3b^2 - 10a^2b^3i + 5ab^4 + b^5i \\ &= a^5 - 10a^3b^2 + 5ab^4 + 5a^4bi - 10a^2b^3i + b^5i \\ &= [a^5 - 10a^3b^2 + 5ab^4] + [5a^4b - 10a^2b^3 + b^5]i \\ &= (a^5 - 10a^3b^2 + 5ab^4, 5a^4b - 10a^2b^3 + b^5) \end{aligned}$$

$$\begin{aligned} R(z^5) \\ &= R(a^5 - 10a^3b^2 + 5ab^4, 5a^4b - 10a^2b^3 + b^5) \\ &= (5a^4b - 10a^2b^3 + b^5, a^5 - 10a^3b^2 + 5ab^4) \\ &= [5a^4b - 10a^2b^3 + b^5] + [a^5 - 10a^3b^2 + 5ab^4]i \end{aligned}$$

$$\begin{aligned} (R(z))^5 \\ &= (b + ai)^5 \\ &= [5a^4b - 10a^2b^3 + b^5] + [a^5 - 10a^3b^2 + 5ab^4]i \\ &= R(z^5) \end{aligned}$$

$$R(z^5) = (R(z))^5$$

$$\underline{y = 0}$$

$$R(x, y) = \left(\frac{(1-(0)^2)x+2(0)y}{1+(0)^2}, \frac{((0)^2-1)y+2(0)x}{1+(0)^2} \right)$$

$$R(x, y) = (x, -y)$$

Proof of Lemma 2 Case 6

Let $z = a + bi; (a, b)$

$$\begin{aligned} R(z) \\ &= R(a, b) \\ &= (a, -b) \end{aligned}$$

$$\begin{aligned} |R(z)| \\ &= |(a, -b)| \\ &= \sqrt{a^2 + (-b)^2} \\ &= \sqrt{a^2 + b^2} \\ &= |z| \end{aligned}$$

$$|R(z)| = |z|$$

Proof of Lemma 3 Case 6

$$z^5 = (a^5 - 10a^3b^2 + 5ab^4, 5a^4b - 10a^2b^3 + b^5)$$

$$\begin{aligned} R(z^5) \\ &= R(a^5 - 10a^3b^2 + 5ab^4, 5a^4b - 10a^2b^3 + b^5) \\ &= (a^5 - 10a^3b^2 + 5ab^4, -[5a^4b - 10a^2b^3 + b^5]) \\ &= [a^5 - 10a^3b^2 + 5ab^4] + (-[5a^4b - 10a^2b^3 + b^5])i \end{aligned}$$

$$\begin{aligned} (R(z))^5 \\ &= [a + (-b)i]^5 \\ &= [a^5 - 10a^3b^2 + 5ab^4] + (-[5a^4b - 10a^2b^3 + b^5])i \\ &= R(z^5) \end{aligned}$$

$$R(z^5) = (R(z))^5$$

$$\underline{y = -x}$$

$$R(x, y) = \left(\frac{(1-(-1)^2)x+2(-1)y}{1+(-1)^2}, \frac{((-1)^2-1)y+2(-1)x}{1+(-1)^2} \right)$$

$$R(x, y) = (-y, -x)$$

Proof of Lemma 2 Case 7

Let $z = a + bi; (a, b)$

$$\begin{aligned} R(z) &= R(a, b) \\ &= (-b, -a) \end{aligned}$$

$$\begin{aligned} |R(z)| &= |(-b, -a)| \\ &= \sqrt{(-b)^2 + (-a)^2} \\ &= \sqrt{a^2 + b^2} \\ &= |z| \end{aligned}$$

$$|R(z)| = |z|$$

Proof of Lemma 3 Case 7

$$z^5 = (a^5 - 10a^3b^2 + 5ab^4, 5a^4b - 10a^2b^3 + b^5)$$

$$\begin{aligned} R(z^5) &= R(a^5 - 10a^3b^2 + 5ab^4, 5a^4b - 10a^2b^3 + b^5) \\ &= (-[5a^4b - 10a^2b^3 + b^5], -[a^5 - 10a^3b^2 + 5ab^4]) \\ &= -[5a^4b - 10a^2b^3 + b^5] + (-[a^5 - 10a^3b^2 + 5ab^4])i \end{aligned}$$

$$\begin{aligned} (R(z))^5 &= [(-b) + (-a)i]^5 \\ &= -[5a^4b - 10a^2b^3 + b^5] + (-[a^5 - 10a^3b^2 + 5ab^4])i \\ &= R(z^5) \end{aligned}$$

$$R(z^5) = (R(z))^5$$

$$\underline{x = 0}$$

$$\begin{aligned} R(x, y) &= \lim_{x \rightarrow \infty} \left(\frac{(1-(m)^2)x+2(m)y}{1+(m)^2}, \frac{((m)^2-1)y+2(m)x}{1+(m)^2} \right) \\ &= \lim_{x \rightarrow \infty} \left(\frac{(-(m)^2)x+2(m)y}{(m)^2}, \frac{((m)^2)y+2(m)x}{(m)^2} \right) \\ &= \lim_{x \rightarrow \infty} \left(-x + \frac{2y}{m}, y + \frac{2x}{m} \right) \\ &= (-x, y) \end{aligned}$$

$$R(x, y) = (-x, y)$$

Proof of Lemma 2 Case 8

Let $z = a + bi; (a, b)$

$$\begin{aligned} R(z) &= R(a, b) \\ &= (-a, b) \end{aligned}$$

$$\begin{aligned} |R(z)| &= |(-a, b)| \\ &= \sqrt{(-a)^2 + (b)^2} \\ &= \sqrt{a^2 + b^2} \\ &= |z| \end{aligned}$$

$$|R(z)| = |z|$$

Proof of Lemma 3 Case 8

$$z^5 = (a^5 - 10a^3b^2 + 5ab^4, 5a^4b - 10a^2b^3 + b^5)$$

$$\begin{aligned} R(z^5) &= R(a^5 - 10a^3b^2 + 5ab^4, 5a^4b - 10a^2b^3 + b^5) \\ &= (-[a^5 - 10a^3b^2 + 5ab^4], 5a^4b - 10a^2b^3 + b^5) \\ &= -[a^5 - 10a^3b^2 + 5ab^4] + [5a^4b - 10a^2b^3 + b^5]i \end{aligned}$$

$$\begin{aligned} (R(z))^5 &= (-a + bi)^5 \\ &= -[a^5 - 10a^3b^2 + 5ab^4] + [5a^4b - 10a^2b^3 + b^5]i \\ &= R(z^5) \end{aligned}$$

$$R(z^5) = (R(z))^5$$

$$\mathbf{1.0.5} \quad f(z) = z^6 + c$$

$$f(z) = z^6 + c, y = \tan\left(\frac{2\pi}{5}\right)x$$

$$\begin{aligned} R(x, y) &= \left(\frac{[(1 - \tan^2(\frac{2\pi}{5}))x + 2 \tan(\frac{2\pi}{5})y]}{1 + \tan^2(\frac{2\pi}{5})}, \frac{[\tan^2(\frac{2\pi}{5}) - 1]y + 2 \tan(\frac{2\pi}{5})x}{1 + \tan^2(\frac{2\pi}{5})} \right) \\ &= \left(\frac{[(1 - \tan^2(\frac{2\pi}{5}))x + 2 \tan(\frac{2\pi}{5})y]}{\sec^2(\frac{2\pi}{5})}, \frac{[\tan^2(\frac{2\pi}{5}) - 1]y + 2 \tan(\frac{2\pi}{5})x}{\sec^2(\frac{2\pi}{5})} \right) \end{aligned}$$

Proof of Lemma 2 Case 10

Let $z = a + bi; (a, b)$

$$|R(z)|$$

$$\begin{aligned}
&= |R(a, b)| \\
&= \left| \left(\frac{[(1 - \tan^2(\frac{2\pi}{5}))a + 2 \tan(\frac{2\pi}{5})b]}{\sec^2(\frac{2\pi}{5})}, \frac{[\tan^2(\frac{2\pi}{5}) - 1]b + 2 \tan(\frac{2\pi}{5})a]}{\sec^2(\frac{2\pi}{5})} \right) \right| \\
&= \sqrt{\left(\frac{[(1 - \tan^2(\frac{2\pi}{5}))a + 2 \tan(\frac{2\pi}{5})b]}{\sec^2(\frac{2\pi}{5})} \right)^2 + \left(\frac{[\tan^2(\frac{2\pi}{5}) - 1]b + 2 \tan(\frac{2\pi}{5})a]}{\sec^2(\frac{2\pi}{5})} \right)^2} \\
&= \sqrt{a^2 + b^2} \\
&= |z|
\end{aligned}$$

$$|R(z)| = |z|$$

Proof of Lemma 3 Case 10

$$\begin{aligned}
z^6 &= (a + bi)^6 \\
&= a^6 + 6a^5bi - 15a^4b^2 - 20a^3b^3i + 15a^2b^4 + 6ab^5i - b^6 \\
&= a^6 - 15a^4b^2 + 15a^2b^4 - b^6 + 6a^5bi - 20a^3b^3i + 6ab^5i \\
&= [a^6 - 15a^4b^2 + 15a^2b^4 - b^6] + [6a^5b - 20a^3b^3 + 6ab^5]i \\
&= (a^6 - 15a^4b^2 + 15a^2b^4 - b^6, 6a^5b - 20a^3b^3 + 6ab^5)
\end{aligned}$$

$$\begin{aligned}
R(z^6) &= R(a^6 - 15a^4b^2 + 15a^2b^4 - b^6, 6a^5b - 20a^3b^3 + 6ab^5) \\
&= \left(\frac{[(1 - \tan^2(\frac{2\pi}{5}))](a^6 - 15a^4b^2 + 15a^2b^4 - b^6) + 2 \tan(\frac{2\pi}{5})(6a^5b - 20a^3b^3 + 6ab^5)}{\sec^2(\frac{2\pi}{5})}, \right. \\
&\quad \left. \frac{[\tan^2(\frac{2\pi}{5}) - 1](6a^5b - 20a^3b^3 + 6ab^5) + 2 \tan(\frac{2\pi}{5})(a^6 - 15a^4b^2 + 15a^2b^4 - b^6)}{\sec^2(\frac{2\pi}{5})} \right) \\
&= \frac{[(1 - \tan^2(\frac{2\pi}{5}))](a^6 - 15a^4b^2 + 15a^2b^4 - b^6) + 2 \tan(\frac{2\pi}{5})(6a^5b - 20a^3b^3 + 6ab^5)}{\sec^2(\frac{2\pi}{5})} \\
&\quad + \frac{[\tan^2(\frac{2\pi}{5}) - 1](6a^5b - 20a^3b^3 + 6ab^5) + 2 \tan(\frac{2\pi}{5})(a^6 - 15a^4b^2 + 15a^2b^4 - b^6)}{\sec^2(\frac{2\pi}{5})} i
\end{aligned}$$

$$\begin{aligned}
(R(z))^6 &= \left(\frac{[(1 - \tan^2(\frac{2\pi}{5}))a + 2 \tan(\frac{2\pi}{5})b]}{\sec^2(\frac{2\pi}{5})} + \frac{[\tan^2(\frac{2\pi}{5}) - 1]b + 2 \tan(\frac{2\pi}{5})a]}{\sec^2(\frac{2\pi}{5})} i \right)^6 \\
&= \frac{[(1 - \tan^2(\frac{2\pi}{5}))](a^6 - 15a^4b^2 + 15a^2b^4 - b^6) + 2 \tan(\frac{2\pi}{5})(6a^5b - 20a^3b^3 + 6ab^5)}{\sec^2(\frac{2\pi}{5})} \\
&\quad + \frac{[\tan^2(\frac{2\pi}{5}) - 1](6a^5b - 20a^3b^3 + 6ab^5) + 2 \tan(\frac{2\pi}{5})(a^6 - 15a^4b^2 + 15a^2b^4 - b^6)}{\sec^2(\frac{2\pi}{5})} i \\
&= R(z^6)
\end{aligned}$$

$$R(z^6) = (R(z))^6$$

While equality may not seem immediately obvious due to its large computational nature, the corresponding contour plots of $R(z)^6$ and $(R(z))^6$ match, strongly suggesting equality.

